code/ecdsap256/Hacl.Impl.P256.PointDouble.fsti
@@ -9,7 +9,6 @@ open Hacl.Impl.P256.Arithmetics
 
 open Lib.Buffer
 
-(* open Spec.P256.Lemmas *)
 open Hacl.Spec.P256.Definition
 open Hacl.Spec.P256.MontgomeryMultiplication
 open Spec.P256
@@ -26,27 +25,35 @@ open FStar.Mul
 
 #reset-options "--z3rlimit 300" 
 
-(*
-val point_double: p: point -> result: point -> tempBuffer: lbuffer uint64 (size 88) -> Stack unit
+val point_double: #c: curve -> p: point c -> result: point c -> tempBuffer: lbuffer uint64 (size (getCoordinateLenU64 c * 22)) -> Stack unit
   (requires fun h -> live h p /\ live h tempBuffer /\ live h result /\
     disjoint p tempBuffer /\ disjoint result tempBuffer /\
     eq_or_disjoint p result /\
-    as_nat h (gsub p (size 8) (size 4)) < prime256 /\ 
-    as_nat h (gsub p (size 0) (size 4)) < prime256 /\ 
-    as_nat h (gsub p (size 4) (size 4)) < prime256)
-  (ensures fun h0 _ h1 -> modifies (loc tempBuffer |+| loc result)  h0 h1 /\  
-    as_nat h1 (gsub result (size 8) (size 4)) < prime256 /\ 
-    as_nat h1 (gsub result (size 0) (size 4)) < prime256 /\ 
-    as_nat h1 (gsub result (size 4) (size 4)) < prime256 /\
     (
-      let x, y, z = gsub p (size 0) (size 4),  gsub p (size 4) (size 4), gsub p (size 8) (size 4) in 
-      let x3, y3, z3 = gsub result (size 0) (size 4), gsub result (size 4) (size 4), gsub result (size 8) (size 4) in 
-      
-      let xD, yD, zD = fromDomain_ (as_nat h0 x), fromDomain_ (as_nat h0 y), fromDomain_ (as_nat h0 z) in 
-      let x3D, y3D, z3D = fromDomain_ (as_nat h1 x3), fromDomain_ (as_nat h1 y3), fromDomain_ (as_nat h1 z3) in
-      
-      let xN, yN, zN = _point_double #P256 (xD, yD, zD) in 
-      x3D == xN /\ y3D == yN /\ z3D == zN
+      let prime = getPrime c in 
+      let len = getCoordinateLenU64 c in
+      as_nat c h (gsub p (size 0) (size len)) < prime /\ 
+      as_nat c h (gsub p (size len) (size len)) < prime /\
+      as_nat c h (gsub p (size (2 * len)) (size len)) < prime
+    )
   )
-) 
- *)
+  (ensures fun h0 _ h1 -> modifies (loc tempBuffer |+| loc result)  h0 h1 /\  
+    (
+      let prime = getPrime c in 
+      let len = getCoordinateLenU64 c in 
+      
+      as_nat c h1 (gsub result (size 0) (size len)) < prime /\ 
+      as_nat c h1 (gsub result (size len) (size len)) < prime /\
+      as_nat c h1 (gsub result (size (2 * len)) (size len)) < prime /\ 
+      
+      (
+	let x, y, z = gsub p (size 0) (size len), gsub p (size len) (size len), gsub p (size (2 * len)) (size len) in 
+	let x3, y3, z3 = gsub result (size 0) (size len), gsub result (size len) (size len), gsub result (size (2 * len)) (size len) in 
+      
+	let xD, yD, zD = fromDomain_ (as_nat c h0 x), fromDomain_ (as_nat c h0 y), fromDomain_ (as_nat c h0 z) in 
+	let x3D, y3D, z3D = fromDomain_ (as_nat c h1 x3), fromDomain_ (as_nat c h1 y3), fromDomain_ (as_nat c h1 z3) in
+	let xN, yN, zN = _point_double #c (xD, yD, zD) in 
+	x3D == xN /\ y3D == yN /\ z3D == zN
+      )
+    ) 
+  )
